src/SlotsCommon.fsti
@@ -18,14 +18,6 @@ open Utils2
 
 #push-options "--fuel 0 --ifuel 0"
 
-noextract
-let seq_u64_or
-  (s1 s2: Seq.lseq U64.t 4)
-  : Seq.lseq U64.t 4
-  =
-  Seq2.map_seq2_len (fun x y -> U64.logor x y) s1 s2;
-  Seq2.map_seq2 (fun x y -> U64.logor x y) s1 s2
-
 #push-options "--z3rlimit 50"
 let slot_array (size_class: sc) (arr: array U8.t) (pos: U32.t)
   : Pure (array U8.t)
